Add secret key zero knowledge check to boardroom voting

execution/theories/Serializable.v
@@ -3,12 +3,14 @@ This format, SerializedValue, is either a unit/int/bool or a pair/list
 of these. We also define Serializable as a type class capturing that a
 type can be converted from and to this format. *)
 
-From Coq Require Import ZArith.
 Require Import Monads.
 Require Import Containers.
 Require Import Automation.
 Require Import BoundedN.
 From Coq Require Import List.
+From Coq Require Import Psatz.
+From Coq Require Import ZArith.
+From stdpp Require countable.
 
 Import ListNotations.
 
@@ -397,3 +399,158 @@ Notation "'Derive' 'Serializable' rect < c0 , .. , cn >" :=
      | [pairs := ?x |- _] => make_serializable rect x
      end))
     (at level 0, rect at level 10, c0, cn at level 9, only parsing).
+
+Section Countable.
+  Instance SerializedType_interp_EqDecision
+           (t : SerializedType) : stdpp.base.EqDecision (interp_type t).
+  Proof. induction t; typeclasses eauto. Defined.
+  Instance SerializedType_interp_Countable
+           (t : SerializedType) : countable.Countable (interp_type t).
+  Proof. induction t; typeclasses eauto. Defined.
+
+  Global Instance SerializedValue_EqDecision : stdpp.base.EqDecision SerializedValue.
+  Proof.
+    intros x y.
+    destruct x as [xt xv], y as [yt yv].
+    destruct (SerializedType.eq_dec xt yt) as [<-|?]; [|right; congruence].
+    destruct (stdpp.base.decide (xv = yv)).
+    - left.
+      congruence.
+    - right.
+      intros eq.
+      inversion eq.
+      congruence.
+  Defined.
+
+  Instance SerializedType_EqDecision : stdpp.base.EqDecision SerializedType.
+  Proof.
+    intros x y.
+    destruct (SerializedType.eq_dec x y) as [<-|?]; [left|right]; easy.
+  Defined.
+  Fixpoint depth st : nat :=
+    match st with
+    | ser_unit => 1
+    | ser_int => 1
+    | ser_bool => 1
+    | ser_pair x y => S (max (depth x) (depth y))
+    | ser_list x => S (depth x)
+    end.
+  Local Open Scope positive.
+  Fixpoint encode_st_body (st : SerializedType) : positive :=
+    match st with
+    | ser_unit => countable.encode (1, 1)
+    | ser_int => countable.encode (2, 1)
+    | ser_bool => countable.encode (3, 1)
+    | ser_pair x y => countable.encode (4, countable.encode (encode_st_body x, encode_st_body y))
+    | ser_list x => countable.encode (5, encode_st_body x)
+    end.
+  Definition encode_st (st : SerializedType) : positive :=
+    countable.encode (depth st, encode_st_body st).
+
+  Fixpoint decode_st_body (depth : nat) (p : positive) : option SerializedType :=
+    match depth with
+    | 0%nat => None
+    | S depth =>
+      do '(tag, body) <- countable.decode p;
+      match tag with
+      | 1 => ret ser_unit
+      | 2 => ret ser_int
+      | 3 => ret ser_bool
+      | 4 => do '(x, y) <- countable.decode body;
+             do x <- decode_st_body depth x;
+             do y <- decode_st_body depth y;
+             ret (ser_pair x y)
+      | 5 => do x <- decode_st_body depth body;
+             ret (ser_list x)
+      | _ => None
+      end
+    end.
+  Definition decode_st (p : positive) : option SerializedType :=
+    do '(depth, body) <- countable.decode p;
+    decode_st_body depth body.
+
+  Local Open Scope nat.
+  Lemma decode_st_body_encode_st_body (d : nat) (st : SerializedType) :
+    depth st <= d ->
+    decode_st_body d (encode_st_body st) = Some st.
+  Proof.
+    revert st.
+    induction d; intros st dle; cbn in *.
+    - exfalso.
+      induction st; cbn in *; lia.
+    - destruct st; auto; cbn in *.
+      + now rewrite !countable.decode_encode, !IHd by lia.
+      + now rewrite !countable.decode_encode, !IHd by lia.
+  Qed.
+
+  Lemma decode_st_encode_st (st : SerializedType) :
+    decode_st (encode_st st) = Some st.
+  Proof.
+    unfold decode_st, encode_st.
+    rewrite countable.decode_encode; cbn.
+    now apply decode_st_body_encode_st_body.
+  Qed.
+
+  Local Open Scope positive.
+  Instance SerializedType_Countable : countable.Countable SerializedType :=
+    {| countable.encode := encode_st;
+       countable.decode := decode_st;
+       countable.decode_encode := decode_st_encode_st |}.
+
+  Definition encode_sv (sv : SerializedValue) : positive :=
+    countable.encode (ser_value_type sv, countable.encode (ser_value sv)).
+
+  Definition decode_sv (p : positive) : option SerializedValue :=
+    do '(ty, p) <- countable.decode p;
+    do v <- countable.decode p;
+    ret {| ser_value_type := ty; ser_value := v |}.
+
+  Lemma decode_sv_encode_sv (sv : SerializedValue) :
+    decode_sv (encode_sv sv) = Some sv.
+  Proof.
+    unfold decode_sv, encode_sv.
+    rewrite countable.decode_encode; cbn.
+    rewrite countable.decode_encode; cbn.
+    reflexivity.
+  Qed.
+
+  Global Instance SerializedValue_Countable : countable.Countable SerializedValue :=
+    {| countable.encode := encode_sv;
+       countable.decode := decode_sv;
+       countable.decode_encode := decode_sv_encode_sv |}.
+
+  Global Instance SerializableType_EqDecision
+         (A : Type) `{Serializable A} : stdpp.base.EqDecision A.
+  Proof.
+    intros a a'.
+    destruct (stdpp.base.decide (serialize a = serialize a')) as [eq|neq].
+    - left.
+      now apply serialize_injective.
+    - right.
+      intros ->.
+      congruence.
+  Defined.
+
+  Definition encode_serializable_type {A : Type} `{Serializable A} (a : A) : positive :=
+    countable.encode (serialize a).
+
+  Definition decode_serializable_type {A : Type} `{Serializable A} (p : positive) : option A :=
+    countable.decode p >>= deserialize.
+
+  Lemma decode_serializable_type_encode_serializable_type
+        {A : Type} `{Serializable A}
+        (a : A) :
+    decode_serializable_type (encode_serializable_type a) = Some a.
+  Proof.
+    unfold decode_serializable_type, encode_serializable_type.
+    rewrite countable.decode_encode.
+    cbn.
+    now rewrite deserialize_serialize.
+  Qed.
+
+  Global Instance SerializableType_Countable {A : Type} `{Serializable A} :
+    countable.Countable A :=
+    {| countable.encode := encode_serializable_type;
+       countable.decode := decode_serializable_type;
+       countable.decode_encode := decode_serializable_type_encode_serializable_type; |}.
+End Countable.
